+ Seq

Opcodes.fst
@@ -10,22 +10,62 @@ module List = FStar.List.Tot
 (* 76 A9 14 ... 88 AC *)
 
 
+assume val hash_sha256: input : seq nat  -> Tot(r: seq nat{Seq.length r = 32} )
+assume val hash_ripemd160: input : seq nat -> Tot(r: seq nat{Seq.length r = 20} )
+
 (* 118 *)
-
-
-val op_dup : #a: eqtype -> st_before: stackBC a{Stack.length st_before > 0 /\ Stack.capacity st_before > 0}  -> 
-				line_before: seq nat{Seq.length line_before > 0 /\ (Seq.head line_before = 118)}
-				-> Tot (st: stackBC a 
+val op_dup :  st_before: stackBC (seq nat){Stack.length st_before > 0 /\ Stack.capacity st_before > 0}  -> 
+				line_before: seq nat{Seq.length line_before > 0 /\ (Seq.head line_before = 118)} 
+				-> result_before : bool{result_before = true}
+				-> Tot (st: stackBC (seq nat)
 								{Stack.length st > 1 /\ 
 								(Stack.index st 0) = (Stack.index st 1) /\ 
 								Stack.length st = Stack.length st_before + 1}	* 
-						line : seq nat {Seq.length line = Seq.length line_before - 1 }) 
+						line : seq nat {Seq.length line = Seq.length line_before - 1 } * result: bool) 
 
-let op_dup #a st_before line_before = 
+let op_dup  st_before line_before result_before = 
 	let pop = Stack.pop st_before in 
 	let element = fst pop in 
 	let stack_after_pop = snd pop in 
 	let stack_push1 = Stack.push stack_after_pop element in 
 	let stack_push2 = Stack.push stack_push1 element in 
-	let line = Seq.tail line_before in (stack_push2, line)
+	let line = Seq.tail line_before in (stack_push2, line, result_before)
 
+val op_hash160 : st_before : stackBC (seq nat){Stack.length st_before > 0} -> 
+				line_before : seq nat {Seq.length line_before > 0 /\ (Seq.head line_before = 169)}
+				-> result_before : bool {result_before = true}
+				-> Tot(st: stackBC (seq nat)
+						{Stack.length st > 0  /\
+						Stack.index st 0 = (hash_ripemd160(hash_sha256 (Stack.index st_before 0))) /\
+						Stack.length st = Stack.length st_before} * 
+					line : seq nat {Seq.length line = Seq.length line_before - 1} * result: bool)
+
+let op_hash160 st_before line_before result_before = 
+		let pop = Stack.pop st_before in 
+		let element = fst pop in 
+		let stack_after_pop = snd pop in 
+		let element = hash_ripemd160(hash_sha256 element) in 
+		let stack_push1 = Stack.push stack_after_pop element in 
+		let line = Seq.tail line_before in (stack_push1, line, result_before)
+
+(* 1 - 75*)
+
+(*val split: #a:Type -> s:seq a -> i:nat{(0 <= i /\ i <= length s)} -> Tot (seq a * seq a) *)
+val op_push : st_before: stackBC (seq nat){ capacity st_before > 0}
+				-> line_before : seq nat {Seq.length line_before > 0 /\ 
+											Seq.length line_before > 1 + (Seq.head line_before)} ->
+				result_before: bool{result_before = true}
+				-> Tot(st: stackBC (seq nat) {Stack.length st > 0 /\ 
+		Seq.length (Stack.index st 0) = Seq.head line_before} *  
+		line : seq nat {Seq.length line = Seq.length line_before -1 - (Seq.head line_before)}
+		* result: bool
+	)
+
+let op_push st_before line_before result_before = 
+		let number_of_bytes = Seq.head line_before in 
+		let line_before = Seq.split line_before 1 in 
+		let line = snd line_before in 
+		let line = Seq.split line number_of_bytes in 
+		let element = fst line in 
+		let stack_push1 = Stack.push st_before element  in 
+		(stack_push1, snd line, result_before)
